@prefix dc: <http://purl.org/dc/elements/1.1/> .
@prefix dcterms: <http://purl.org/dc/terms/> .
@prefix rdf: <http://www.w3.org/1999/02/22-rdf-syntax-ns#> .
@prefix rdfs: <http://www.w3.org/2000/01/rdf-schema#> .
@prefix skos: <http://www.w3.org/2004/02/skos/core#> .
@prefix xml: <http://www.w3.org/XML/1998/namespace> .
@prefix xsd: <http://www.w3.org/2001/XMLSchema#> .
@prefix skosxl: <http://www.w3.org/2008/05/skos-xl#> .
@prefix adms: <http://www.w3.org/ns/adms#> .
@prefix vs: <http://www.w3.org/2003/06/sw-vocab-status/ns#> .
@prefix alignment: <http://purl.org/dcx/lrmi-vocabs/alignmentType/> .

alignment: a skos:ConceptScheme ;
    dc:description """Describes the types of relationships between a learning resource and 
        an AlighmentObject."""@en-US ;
    dc:title "LRMI Alignment Type Vocabulary"@en-US ;
    dcterms:created "2015-01-21"^^xsd:date ;
    dcterms:license <http://creativecommons.org/licenses/by/4.0/> ;
    adms:status <http://purl.org/dcx/lrmi-vocabs/docStatus/draft> .    

alignment:assesses: a skos:Concept ;
    skos:prefLabel "assesses"@en-US ;
    skosxl:preflabel alignment:label-assesses ;    
    skos:definition """The origin of the association may be used to assess the destination 
        of the association."""@en-US ;
    skos:inScheme alignment: ;
    vs:term_status "unstable" .

alignment:teaches a skos:Concept ;
    skos:prefLabel "teaches"@en-US ;
    skosxl:preflabel alignment:label-teaches ;    
    skos:definition """The resource or method at the origin of the association may be used 
        to teach the competency at the destination of the association."""@en-US ;
    skos:inScheme alignment: ;
    vs:term_status "unstable" .            

alignment:requires a skos:Concept ;
    skos:prefLabel "requires"@en-US ;
    skosxl:preflabel alignment:label-requires ;    
    skos:definition """The origin of the association requires the destination of the association 
        to support its function, delivery, or coherence."""@en-US ;
    skos:inScheme alignment: ;    
    vs:term_status "unstable" .    
   

alignment:textComplexity a skos:Concept ;
    skos:prefLabel "text complexity"@en-US ;
    skosxl:preflabel alignment:label-textComplexity ;    
    skos:definition """The destination of the association defines a level or range, measuring 
        the ease in which text can be read and understood, for text used within the resource at 
        the origin of the association."""@en-US ;
    skos:inScheme alignment: ;     
    vs:term_status "unstable" .

alignment:readingLevel a skos:Concept ;
    skos:prefLabel "reading level"@en-US ;
    skosxl:preflabel alignment:label-readingLevel ;    
    skos:definition """The destination of the association defines a level or range of ability 
        expected for a person using the resource at the origin of the association."""@en-US ;
    skos:inScheme alignment: ;     
    vs:term_status "unstable" .

alignment:educationalSubject a skos:Concept ;
    skos:prefLabel "educational subject"@en-US ;
    skosxl:preflabel alignment:label-educationalSubject ;    
    skos:definition """The destination of the association defines a topic or subject from a 
        controlled vocabulary."""@en-US ;
    skos:inScheme alignment: ;
    vs:term_status "unstable" .  
    
alignment:cognitiveComplexity: a skos:Concept ;
    skos:prefLabel "cognitive complexity"@en-US ;
    skosxl:preflabel alignment:label-cognitiveComplexity ;    
    skos:definition """@@@."""@en-US ;
    skos:inScheme alignment: ;
    vs:term_status "unstable" .      

alignment:educationalLevel a skos:Concept ;
    skos:prefLabel "educational level"@en-US ;
    skosxl:preflabel alignment:label-educationalLevel ;    
    skos:definition """he destination of the association defines an education level from a 
        controlled vocabulary."""@en-US ;
    skos:inScheme alignment: ;
    vs:term_status "unstable" .         
    
#============================= 
# EXTENDED LABELS
#=============================    
    
alignment:label-assesses a skosxl:label ;
    skosxl:literalForm "assesses"@en-US .
    
alignment:label-cognitiveComplexity a skosxl:label ;
    skosxl:literalForm "cognitive complexity"@en-US .     
    
alignment:label-teaches a skosxl:label ;
    skosxl:literalForm "teaches"@en-US .   
        
alignment:label-requires a skosxl:label ;
    skosxl:literalForm "requires"@en-US .   
        
alignment:label-textComplexity a skosxl:label ;
    skosxl:literalForm "text complexity"@en-US .
        
alignment:label-readingLevel a skosxl:label ;
    skosxl:literalForm "reading level"@en-US .  
        
alignment:label-educationalSubject a skosxl:label ;
    skosxl:literalForm "educational subject"@en-US .
        
alignment:label-educationalLevel a skosxl:label ;
    skosxl:literalForm "educational level"@en-US .                             
