@prefix dc: <http://purl.org/dc/elements/1.1/> .
@prefix dcterms: <http://purl.org/dc/terms/> .
@prefix rdf: <http://www.w3.org/1999/02/22-rdf-syntax-ns#> .
@prefix rdfs: <http://www.w3.org/2000/01/rdf-schema#> .
@prefix skos: <http://www.w3.org/2004/02/skos/core#> .
@prefix xml: <http://www.w3.org/XML/1998/namespace> .
@prefix xsd: <http://www.w3.org/2001/XMLSchema#> .
@prefix skosxl: <http://www.w3.org/2008/05/skos-xl#> .
@prefix adms: <http://www.w3.org/ns/adms#> .
@prefix vs: <http://www.w3.org/2003/06/sw-vocab-status/ns#> .
@prefix alignment: <http://purl.org/dcx/lrmi-vocabs/alignmentType/> .

alignment: a skos:ConceptScheme ;
    dc:description """Describes the types of relationships between a learning resource 
        and an AlighmentObject."""@en ;
    dc:title "LRMI Alignment Type Vocabulary"@en ;
    dcterms:created "2015-01-21"^^xsd:date ;
    dcterms:license <http://creativecommons.org/licenses/by/4.0/> ;
    adms:status <http://purl.org/dcx/lrmi-vocabs/docStatus/draft> .    

alignment:assesses: a skos:Concept ;
    skos:inScheme alignment: ;
    skos:prefLabel "assesses"@en ;
    skosxl:preflabel alignment:label-assesses ;
    skos:definition """The resource being described evaluates learner achivement of the competency 
        being referenced."""@en;    
    vs:term_status "unstable" . 

alignment:teaches a skos:Concept ;
    skos:inScheme alignment: ;
    skos:prefLabel "teaches"@en ;
    skosxl:preflabel alignment:label-teaches ;
    skos:definition """The resource being described instructs, imparts or conveys the 
        knowledge, skill, or habit of mind required by the competency being referenced"""@en;     
    vs:term_status "unstable" .         

alignment:requires a skos:Concept ;
    skos:inScheme alignment: ;
    skos:prefLabel "requires"@en ;
    skosxl:preflabel alignment:label-requires ;
    skos:definition """A resource necessary to the effective use or intended outcome of the 
        resource being described."""@en;    
    vs:term_status "unstable" .    

alignment:textComplexity a skos:Concept ;
    skos:inScheme alignment: ;
    skos:prefLabel "text complexity"@en ;
    skosxl:preflabel alignment:label-textComplexity ;
    skos:definition "A measure of the textual difficulty of the resource being described."@en;    
    vs:term_status "unstable" .    

alignment:readingLevel a skos:Concept ;
    skos:inScheme alignment: ;
    skos:prefLabel "reading level"@en ;
    skosxl:preflabel alignment:label-readingLevel ;
    vs:term_status "unstable" .    

alignment:educationalSubject a skos:Concept ;
    skos:inScheme alignment: ;
    skos:prefLabel "educational subject"@en ;
    skosxl:preflabel alignment:label-educationalSubject ;
    vs:term_status "unstable" .     

alignment:educationalLevel a skos:Concept ;
    skos:inScheme alignment: ;
    skos:prefLabel "educational level"@en ;
    skosxl:preflabel alignment:label-educationalLevel ;
    skos:definition """A class of entity, defined in terms of progression through an educational 
        or training context, for which the described resource is intended."""@en ;
    vs:term_status "unstable" .    
    
#============================= 
# EXTENDED LABELS
#=============================    
    
alignment:label-assesses a skosxl:label ;
    skosxl:literalForm "assesses"@en . 
    
alignment:label-teaches a skosxl:label ;
    skosxl:literalForm "teaches"@en .   
        
alignment:label-requires a skosxl:label ;
    skosxl:literalForm "requires"@en .   
        
alignment:label-textComplexity a skosxl:label ;
    skosxl:literalForm "text complexity"@en .
        
alignment:label-readingLevel a skosxl:label ;
    skosxl:literalForm "reading level"@en .  
        
alignment:label-educationalSubject a skosxl:label ;
    skosxl:literalForm "educational subject"@en .
        
alignment:label-educationalLevel a skosxl:label ;
    skosxl:literalForm "educational level"@en .                             
