@prefix audType: <http://purl.org/dcx/lrmiAudienceType/> .
@prefix skos: <http://www.w3.org/2004/02/skos/core#> .
@prefix schema: <http://schema.org/> .
@prefix rdf: <http://www.w3.org/1999/02/22-rdf-syntax-ns#> .
@prefix rdfs: <http://www.w3.org/2000/01/rdf-schema#> .
@prefix xsd: <http://www.w3.org/2001/XMLSchema#> .
@prefix owl: <http://www.w3.org/2002/07/owl#> .
@prefix dct: <http://purl.org/dc/terms/> .
@prefix dc: <http://purl.org/dc/elements/1.1/> .
@prefix foaf: <http://xmlns.com/foaf/0.1/> .

<http://purl.org/dcx/lrmiAudienceType/> rdf:type skos:ConceptScheme;
  dct:title "LRMI Audience Type Vocabulary";
  dc:creator "LRMI Task Group (DCMI)"@en;
  dct:created "2015-01-21"^^xsd:date ;
  dct:license <http://creativecommons.org/licenses/by/4.0/>.
  
audType:9b8b1d37-cbe3-472b-9bc6-eb67693006c8 rdf:type skos:Concept;
  skos:prefLabel "administrator"@en;
  skos:prefLabel "administrateur"@fr;
  skos:prefLabel "administrador"@es;
  skos:definition "A district or school level person of authority and responsibility"@en;
  skos:definition "Una persona distrito o la escuela de nivel de autoridad y responsabilidad"@es;
  skos:definition "Une personne au niveau du district ou de l'école de l'autorité et de la responsabilité"@fr;
  skos:inScheme <http://purl.org/dcx/lrmiAudienceType/>.

audType:93184541-bbcd-4613-844d-0d54e0b21c0d rdf:type skos:Concept;
  skos:prefLabel "mentor"@en;
  skos:altLabel "guide"@en, "guider"@fr, "guiar"@es;
  skos:definition "Someone who advises, trains, supports, and/or guides."@en;
  skos:inScheme <http://purl.org/dcx/lrmiAudienceType/>.

audType:9e8b8d04-47d8-4201-962c-19a3c8b1f7cf rdf:type skos:Concept;
  skos:prefLabel "general public"@en;
  skos:definition "The Public at large."@en;
  skos:inScheme <http://purl.org/dcx/lrmiAudienceType/>.

audType:17c78c23-616f-468e-beb1-9aaf5181b14f rdf:type skos:Concept;
  skos:prefLabel "parent"@en;
  skos:definition "A parent or legal guardian."@en;
  skos:inScheme <http://purl.org/dcx/lrmiAudienceType/>.  
       
audType:457df3c5-247e-445a-bf3d-3145ce795961 rdf:type skos:Concept;
  skos:prefLabel "professional"@en;
  skos:definition "Someone already practicing a profession; an industry partner, or professional development trainer."@en;
  skos:inScheme <http://purl.org/dcx/lrmiAudienceType/>.  
       
audType:fc35bd68-f301-4ac2-8bdc-f965d2a26a0f rdf:type skos:Concept;
  skos:prefLabel "student"@en;
  skos:definition "The learner."@en;
  skos:narrower lrmiType:a6760d5b-97b2-46ab-8b83-80ccd3f789d9;
  skos:inScheme <http://purl.org/dcx/lrmiAudienceType/>.
  
audType:a6760d5b-97b2-46ab-8b83-80ccd3f789d9 rdf:type skos:Concept;
  skos:prefLabel "peer/tutor"@en;
  skos:definition "The peer learner serving as tutor of another learner."@en;
  skos:inScheme <http://purl.org/dcx/lrmiAudienceType/>.    
       
audType:e9d882e6-e1b8-495c-803f-12fb832cc557 rdf:type skos:Concept;
  skos:prefLabel "teacher/education specialist"@en;
  skos:definition "A certified person directly involved with student instruction."@en;
  skos:inScheme <http://purl.org/dcx/lrmiAudienceType/>.
