@prefix audRole: <http://purl.org/dcx/lrmi-vocabs/educationalAudienceRole/> .
@prefix skos: <http://www.w3.org/2004/02/skos/core#> .
@prefix schema: <http://schema.org/> .
@prefix rdf: <http://www.w3.org/1999/02/22-rdf-syntax-ns#> .
@prefix rdfs: <http://www.w3.org/2000/01/rdf-schema#> .
@prefix xsd: <http://www.w3.org/2001/XMLSchema#> .
@prefix owl: <http://www.w3.org/2002/07/owl#> .
@prefix dct: <http://purl.org/dc/terms/> .
@prefix dc: <http://purl.org/dc/elements/1.1/> .
@prefix foaf: <http://xmlns.com/foaf/0.1/> .
@prefix vs: <http://www.w3.org/2003/06/sw-vocab-status/ns#> .

<http://purl.org/dcx/lrmi-vocabs/educationalAudienceRole/> rdf:type skos:ConceptScheme;
  dct:title "LRMI Educational Audience Role Vocabulary";
  dc:creator "LRMI Task Group (DCMI)"@en;
  dct:created "2015-01-21"^^xsd:date ;
  dct:license <http://creativecommons.org/licenses/by/4.0/>.
  
audRole:001 rdf:type skos:Concept;
  skos:prefLabel "administrator"@en;
  skos:prefLabel "administrateur"@fr;
  skos:prefLabel "administrador"@es;
  skos:definition "A district or school level person of authority and responsibility"@en;
  skos:definition "Una persona distrito o la escuela de nivel de autoridad y responsabilidad"@es;
  skos:definition "Une personne au niveau du district ou de l'école de l'autorité et de la responsabilité"@fr;
  skos:inScheme <http://purl.org/dcx/lrmi-vocabs/educationalAudienceRole/>;
  vs:term_status "unstable" .

audRole:002 rdf:type skos:Concept;
  skos:prefLabel "mentor"@en;
  skos:altLabel "guide"@en, "guider"@fr, "guiar"@es;
  skos:definition "Someone who advises, trains, supports, and/or guides."@en;
  skos:inScheme <http://purl.org/dcx/lrmi-vocabs/educationalAudienceRole/>;
  vs:term_status "unstable" .

audRole:003 rdf:type skos:Concept;
  skos:prefLabel "general public"@en;
  skos:definition "The Public at large."@en;
  skos:inScheme <http://purl.org/dcx/lrmi-vocabs/educationalAudienceRole/>;
  vs:term_status "unstable" .

audRole:004 rdf:type skos:Concept;
  skos:prefLabel "parent"@en;
  skos:definition "A parent or legal guardian."@en;
  skos:inScheme <http://purl.org/dcx/lrmi-vocabs/educationalAudienceRole/>;
  vs:term_status "unstable" .
       
audRole:005 rdf:type skos:Concept;
  skos:prefLabel "professional"@en;
  skos:definition "Someone already practicing a profession; an industry partner, or professional development trainer."@en;
  skos:inScheme <http://purl.org/dcx/educationalAudienceRole/>;
  vs:term_status "unstable" .
       
audRole:006 rdf:type skos:Concept;
  skos:prefLabel "student"@en;
  skos:definition "The learner."@en;
  skos:narrower audType:007;
  skos:inScheme <http://purl.org/dcx/lrmi-vocabs/educationalAudienceRole/>;
  vs:term_status "unstable" .
  
audRole:007 rdf:type skos:Concept;
  skos:prefLabel "peer/tutor"@en;
  skos:definition "The peer learner serving as tutor of another learner."@en;
  skos:broader audType:006;
  skos:inScheme <http://purl.org/dcx/lrmi/educationalAudienceRole/>;
  vs:term_status "unstable" .
       
audRole:008 rdf:type skos:Concept;
  skos:prefLabel "teacher/education specialist"@en;
  skos:definition "A certified person directly involved with student instruction."@en;
  skos:inScheme <http://purl.org/dcx/lrmi-vocabs/educationalAudienceRole/>;
  vs:term_status "unstable" .
