@prefix dc: <http://dublincore.org/elements/1.1/> .
@prefix dcterms: <http://purl.org/dc/terms/> .
@prefix rdf: <http://www.w3.org/1999/02/22-rdf-syntax-ns#> .
@prefix rdfs: <http://www.w3.org/2000/01/rdf-schema#> .
@prefix skos: <http://www.w3.org/2004/02/skos/core#> .
@prefix skosxl: <http://www.w3.org/2008/05/skos-xl#> .
@prefix edUse: <http://purl.org/dcx/lrmi-vocabs/edUse/> .
@prefix xml: <http://www.w3.org/XML/1998/namespace> .
@prefix xsd: <http://www.w3.org/2001/XMLSchema#> .
@prefix vs: <http://www.w3.org/2003/06/sw-vocab-status/ns#> .
@prefix adms: <http://www.w3.org/ns/adms#> .

# Defines a set of top-level concepts of Educational Use

edUse: a skos:ConceptScheme ;
    dc:title "LRMI Educational Use vocabulary" ;
    dcterms:created "2015-01-21"^^xsd:date ;
    dcterms:license <http://creativecommons.org/licenses/by/4.0/> ;
    adms:status <http://purl.org/dcx/lrmi-vocabs/docStatus/draft> .      

edUse:instruction a skos:Concept ;
    skos:prefLabel "instruction"@en ;
    skosxl:prefLabel edUse:label-instruction ;
    skos:definition """Primary purpose of the resource is to support the instructional 
        process, student learning, or to provide information about the curriculum."""@en ;
    skos:inScheme <http://purl.org/dcx/lrmi-vocabs/edUse/> ;
    dcterms:source <https://ceds.ed.gov/element/001002> ;
    vs:term_status "unstable" .
    
edUse:assessment a skos:Concept ;
    skos:prefLabel "assessment"@en ;
    skosxl:prefLabel edUse:label-assessment ;
    skos:definition """Primary purpose of the resource is to evaluate learning, either 
        before or after instruction occurs."""@en ;
    skos:inScheme <http://purl.org/dcx/lrmi-vocabs/edUse/> ;
    dcterms:source <https://ceds.ed.gov/element/001002> ;
    vs:term_status "unstable" .   

edUse:professionalDevelopment a skos:Concept ;
    skos:prefLabel "professional development"@en ;
    skosxl:prefLabel edUse:label-professionalDevelopment ;
    skos:definition """Primary purpose of the resource is to provide instruction for a teacher 
        or other education professional."""@en ;
    skos:inScheme <http://purl.org/dcx/lrmi-vocabs/edUse/> ;
    dcterms:source <https://ceds.ed.gov/element/001002> ;  
    vs:term_status "unstable" .
    
# EXTENDED LABELS    

edUse:label-instruction a skosxl:label ;
    skosxl:literalForm "instruction"@en .
        
edUse:label-assessment a skosxl:label ;
    skosxl:literalForm "assessment"@en .
    
edUse:label-professionalDevelopment a skosxl:label ;
    skosxl:literalForm "professional development"@en .
