@prefix dc: <http://dublincore.org/elements/1.1/> .
@prefix dcterms: <http://purl.org/dc/terms/> .
@prefix rdf: <http://www.w3.org/1999/02/22-rdf-syntax-ns#> .
@prefix rdfs: <http://www.w3.org/2000/01/rdf-schema#> .
@prefix skos: <http://www.w3.org/2004/02/skos/core#> .
@prefix xml: <http://www.w3.org/XML/1998/namespace> .
@prefix xsd: <http://www.w3.org/2001/XMLSchema#> .

# Defines a set of top-level concepts of Educational Use

<http://purl.org/dcx/lrmi-vocabs/edUse/> a skos:ConceptScheme ;
    dc:title "LRMI Educational Use vocabulary" .

<http://purl.org/dcx/lrmi-vocabs/edUse/001> a skos:Concept ;
    skos:prefLabel "instruction"@en ;
    skos:definition "Primary purpose of the resource is to support the instructional process, student learning, or to provide information about the curriculum."@en ;
    skos:inScheme <http://purl.org/dcx/lrmi-vocabs/edUse/> ;
    skos:note "Based on the CEDS Learning Resource Educational Use term \"Curriculum/Instruction\" at https://ceds.ed.gov/element/001002."@en .
    
<http://purl.org/dcx/lrmi-vocabs/edUse/002> a skos:Concept ;
    skos:prefLabel "assessment"@en ;
    skos:definition "Primary purpose of the resource is to evaluate learning, either before or after instruction occurs."@en ;
    skos:inScheme <http://purl.org/dcx/lrmi-vocabs/edUse/> ;
    skos:note "Based on the CEDS Learning Resource Educational Use term \"Assessment\" at https://ceds.ed.gov/element/001002."@en .

<http://purl.org/dcx/lrmi-vocabs/edUse/003> a skos:Concept ;
    skos:prefLabel "professional development"@en ;
    skos:definition "Primary purpose of the resource is to provide instruction for a teacher or other education professional."@en ;
    skos:inScheme <http://purl.org/dcx/lrmi-vocabs/edUse/> ;
    skos:note "Based on the CEDS Learning Resource Educational Use term \"Professional Development\" at https://ceds.ed.gov/element/001002."@en .  
