@prefix dc: <http://purl.org/dc/elements/1.1/> .
@prefix dcterms: <http://purl.org/dc/terms/> .
@prefix rdf: <http://www.w3.org/1999/02/22-rdf-syntax-ns#> .
@prefix rdfs: <http://www.w3.org/2000/01/rdf-schema#> .
@prefix skos: <http://www.w3.org/2004/02/skos/core#> .
@prefix skosxl: <http://www.w3.org/2008/05/skos-xl#> .
@prefix xml: <http://www.w3.org/XML/1998/namespace> .
@prefix xsd: <http://www.w3.org/2001/XMLSchema#> .
@prefix vann: <http://purl.org/vocab/vann/> .
@prefix vs: <http://www.w3.org/2003/06/sw-vocab-status/ns#> .
@prefix adms: <http://www.w3.org/ns/adms#> .
@prefix resourceType: <http://purl.org/dcx/lrmi-vocabs/learningResourceType/> .

resourceType: a skos:ConceptScheme ;
    dc:title "LRMI Learning Resource Type Vocabulary"@en ;
    dc:description """The predominate genre, type or kind characterizing the learning 
        resource."""@en ;
    dc:source """Based in part on the CEDS Learning Resource Type vocabulary found at 
        https://ceds.ed.gov/element/000928"""@en ;
    adms:status <http://purl.org/dcx/lrmi-vocabs/docStatus/draft> .

resourceType:alternateAssessment a skos:Concept ;
    skos:prefLabel "alternate assessment"@en ;
    skosxl:prefLabel resourceType:label-alternateAssessment ;    
    skos:definition """An assessment that is used to evaluate the performance of students 
        who are unable to participate in general state assessments even with 
        accommodations."""@en ;
    skos:inScheme resourceType: ;
    dcterms:source <https://ceds.ed.gov/element/000928#AlternateAssessment> ;
    vs:term_status "unstable" .
    
resourceType:assessmentItem a skos:Concept ;
    skos:prefLabel "assessment item"@en ;
    skosxl:prefLabel resourceType:label-assessmentItem ; 
    skos:definition """A specific prompt, that defines a question or protocol for a 
        measurable activity that triggers a response from a person used to determine 
        whether the person has mastered a learning objective."""@en ;
    skos:inScheme resourceType: ;
    dcterms:source <https://ceds.ed.gov/element/000928#AssessmentItem> ;
    vs:term_status "unstable" .
       
resourceType:course a skos:Concept ;
    skos:prefLabel "course"@en ;
    skosxl:prefLabel resourceType:label-course ; 
    skos:definition """A series of units and lessons used to teach the skills and 
        knowledge required by its curriculum."""@en ;
    skos:inScheme resourceType: ;
    dcterms:source <https://ceds.ed.gov/element/000928#Course> ;
    vs:term_status "unstable" .

resourceType:demonstration-simulation a skos:Concept ;
    skos:prefLabel "demonstration/simulation"@en ;
    skosxl:prefLabel resourceType:label-demonstration-simulation ; 
    skos:definition "An imitation or modeling of a real-world process."@en ;
    skos:inScheme resourceType: ;
    dcterms:source <https://ceds.ed.gov/element/000928#DemonstrationSimulation> ;
    vs:term_status "unstable" .
    
resourceType:educatorCurriculum a skos:Concept ;
    skos:prefLabel "educator curriculum Guide"@en ;
    skosxl:prefLabel resourceType:label-educatorCurriculum ;
    skos:definition """A document that defines what concepts should be taught 
        and/or how a concept should be taught effectively."""@en ;
    skos:inScheme resourceType: ;
    dcterms:source <https://ceds.ed.gov/element/000928#EducatorCurriculumGuide> ;
    vs:term_status "unstable" .
    
resourceType:formativeAssessment a skos:Concept ;
    skos:prefLabel "formative sssessment"@en ;
    skosxl:prefLabel resourceType:label-formativeAssessment ;
    skos:definition """A process used by teachers and students during instruction 
        that provides feedback to adjust ongoing teaching and learning to improve 
        students' achievement of intended instructional outcomes. (CCSSO FAST 
        SCASS, 2006)"""@en ;
    skos:inScheme resourceType: ;
    dcterms:source <https://ceds.ed.gov/element/000928#FormativeAssessment> ;
    vs:term_status "unstable" .

resourceType:images-visuals a skos:Concept ;
    skos:prefLabel "images/visuals"@en ;
    skosxl:prefLabel resourceType:label-images-visuals ;
    skos:definition """Visual media, including but not limited to pictures, graphics, 
        diagrams, figures, illustrations, charts, and maps."""@en ;
    skos:inScheme resourceType: ;
    dcterms:source <https://ceds.ed.gov/element/000928#ImagesVisuals> ;
    vs:term_status "unstable" .
    
resourceType:interim-summativeAssessment a skos:Concept ;
    skos:prefLabel "interim/summative assessment"@en ;
    skosxl:prefLabel resourceType:label-interim-summativeAssessment ;
    skos:definition """An assessment instrument used to evaluate student learning 
        at the end of an instructional unit by comparing it against some standard 
        or benchmark. A learning resource of this typemay be an \"assessment form,\" 
        i.e. one instance of the assessment instrument that can equate scores with 
        another instance of the same assessment."""@en ;
    skos:inScheme resourceType: ;
    dcterms:source <https://ceds.ed.gov/element/000928#InterimSummativeAssessment> ;
    vs:term_status "unstable" .    

resourceType:learningActivity a skos:Concept ;
    skos:prefLabel "learning activity"@en ;
    skosxl:prefLabel resourceType:label-learningActivity ;
    skos:definition """Activities engaged in by the learner for the purpose of 
        acquiring certain skills, concepts, or knowledge, whether guided by an 
        instructor or not. A Lesson may define one or more learning activities."""@en ;
    skos:inScheme resourceType: ;
    dcterms:source <https://ceds.ed.gov/element/000928#LearningActivity> ;
    vs:term_status "unstable" .    

resourceType:lesson a skos:Concept ;
    skos:prefLabel "lesson"@en ;
    skosxl:prefLabel resourceType:label-lesson ;
    skos:definition """A detailed description of the course of instruction for a short 
    period of time that is used by a teacher to guide class instruction.  A Unit 
    contains one or more lessons."""@en ;
    skos:inScheme resourceType: ;
    dcterms:source <https://ceds.ed.gov/element/000928#Lesson> ;
    vs:term_status "unstable" .    

resourceType:primarySource a skos:Concept ;
    skos:prefLabel "primary source"@en ;
    skosxl:prefLabel resourceType:label-primarySource ;
    skos:definition """An artifact, document, recording, or other source of information 
        that was created at the time under study and provides first-hand testimony or 
        direct evidence concerning a topic under investigation."""@en ;
    skos:inScheme resourceType: ;
    dcterms:source <https://ceds.ed.gov/element/000928#PrimarySource> ;
    vs:term_status "unstable" .         

resourceType:rubricScoringGuide a skos:Concept ;
    skos:prefLabel "rubric scoring guide"@en ;
    skosxl:prefLabel resourceType:label-rubricScoringGuide ;
    skos:definition """A document or guide that is used to delineate consistent criteria 
        for grading."""@en ;
    skos:inScheme resourceType: ;
    dcterms:source <https://ceds.ed.gov/element/000928#RubricScoringGuide> ;
    vs:term_status "unstable" .

resourceType:selfAssessment a skos:Concept ;
    skos:prefLabel "self assessment"@en ;
    skosxl:prefLabel resourceType:label-selfAssessment ;
    skos:definition """An assessment in which the user gathers information about and 
        reflects on his or her own knowledge, skills, learning, or attitudes."""@en ;
    skos:inScheme resourceType: ;
    dcterms:source <https://ceds.ed.gov/element/000928#SelfAssessment> ;
    vs:term_status "unstable" .

resourceType:text a skos:Concept ;
    skos:prefLabel "text"@en ;
    skosxl:prefLabel resourceType:label-text ;
    skos:definition "The body of a printed work, to include reading passages."@en ;
    skos:inScheme resourceType: ;
    dcterms:source <https://ceds.ed.gov/element/000928#Text> ;
    vs:term_status "unstable" . 

resourceType:textbook a skos:Concept ;
    skos:prefLabel "textbook"@en ;
    skosxl:prefLabel resourceType:label-textbook ;
    skos:definition """A book used as a standard source of information on a particular 
        subject."""@en ;
    skos:inScheme resourceType: ;
    dcterms:source <https://ceds.ed.gov/element/000928#Textbook> ;
    vs:term_status "unstable" .       
 
resourceType:unit a skos:Concept ;
    skos:prefLabel "unit"@en ;
    skosxl:prefLabel resourceType:label-unit ;
    skos:definition """A long-range plan of instruction on a particular concept; it 
        contains multiple lessons that are related."""@en ;
    skos:inScheme resourceType: ;
    dcterms:source <https://ceds.ed.gov/element/000928#Unit> ;
    vs:term_status "unstable" .
    
#============================= 
# EXTENDED LABELS
#=============================    
    
resourceType:label-alternateAssessment a skosxl:label ;
    skosxl:literalForm "alternate assessment"@en .
        
resourceType:label-assessmentItem a skosxl:label ;
    skosxl:literalForm "assessment item"@en . 
        
resourceType:label-course a skosxl:label ;
    skosxl:literalForm "course"@en .
         
resourceType:label-demonstration-simulation a skosxl:label ;
    skosxl:literalForm "demonstration/simulation"@en .
         
resourceType:label-educatorCurriculum a skosxl:label ;
    skosxl:literalForm "educator curriculum"@en .
         
resourceType:label-formativeAssessment a skosxl:label ;
    skosxl:literalForm "formative assessment"@en .
         
resourceType:label-images-visuals a skosxl:label ;
    skosxl:literalForm "@@@"@en .
         
resourceType:label-interim-summativeAssessment a skosxl:label ;
    skosxl:literalForm "interim/summative assessment"@en .
         
resourceType:label-learningActivity a skosxl:label ;
    skosxl:literalForm "learning activity"@en .
         
resourceType:label-lesson a skosxl:label ;
    skosxl:literalForm "lesson"@en .
         
resourceType:label-primarySource a skosxl:label ;
    skosxl:literalForm "primary source"@en .
         
resourceType:label-rubricScoringGuide a skosxl:label ;
    skosxl:literalForm "rubric scoring guide"@en .
         
resourceType:label-selfAssessment a skosxl:label ;
    skosxl:literalForm "self assessment"@en .
         
resourceType:label-text a skosxl:label ;
    skosxl:literalForm "text"@en .
         
resourceType:label-textbook a skosxl:label ;
    skosxl:literalForm "textbook"@en .
         
resourceType:label-unit a skosxl:label ;
    skosxl:literalForm "unit"@en .      
